Merge branch 'master' of file://///afs/csail.mit.edu/group/plv/git/adt-synthesis

ADTRefinement/Core.v
@@ -71,10 +71,9 @@ Notation "c ↝ v" := (computes_to c v) (at level 70).
     used to be callable should still be callable, and we don't care
     about the other methods. *)
 
-Inductive refineADT {Sig} :
-  ADT Sig -> ADT Sig -> Prop :=
+Inductive refineADT {Sig} (A B : ADT Sig) : Prop :=
 | refinesADT :
-    forall A B SiR,
+    forall SiR,
       (forall idx : MutatorIndex Sig,
          @refineMutator
                      (Rep A) (Rep B) SiR
@@ -93,3 +92,12 @@ Inductive refineADT {Sig} :
     into [refine], so that we can rewrite with lemmas about [refine]. *)
 Arguments refineMutator / .
 Arguments refineObserver / .
+
+(** If our goal is a [Prop], then we can extract the simulation relation. *)
+Definition refineADT_SiR_elim {Sig} {A B : ADT Sig} (P : Prop)
+           (H : (Rep A -> Rep B -> Prop) -> P)
+           (H' : refineADT A B)
+: P
+  := match H' with
+       | refinesADT SiR _ _ => H SiR
+     end.
