ADTRefinement/GeneralBuildADTRefinements.v
@@ -129,40 +129,92 @@ Section BuildADTRefinements.
 
   Hint Resolve In_obsSigs.
 
-  Lemma refineADT_BuildADT_ReplaceObserver
+  Lemma refineADT_BuildADT_ReplaceObserver_generic_ex
             (Rep : Type)
-            (SiR : Rep -> Rep -> Prop)
             (mutSigs : list mutSig)
             (obsSigs : list obsSig)
             (mutDefs : ilist (@mutDef Rep) mutSigs)
             (obsDefs : ilist (@obsDef Rep) obsSigs)
             (idx : BoundedString (List.map obsID obsSigs))
-            (newDef : obsDef (nth (findIndex obsSig_eq obsSigs idx) obsSigs _))
-  : (forall mutIdx,
-       refineMutator SiR (getMutDef mutDefs mutIdx) (getMutDef mutDefs mutIdx))
-    -> (forall obsIdx,
-          refineObserver SiR (getObsDef obsDefs obsIdx) (getObsDef obsDefs obsIdx))
-    -> refineObserver SiR
-                  (obsBody (ith obsSig_eq obsDefs idx _
-                                (@Build_obsDef Rep ("null" : rep × () → ()) (fun r _ => ret tt))
-                                ))
-                  (obsBody newDef)
+            (newDef : obsDef (nth (findIndex obsSig_eq obsSigs idx)
+                                  obsSigs ("null" : rep × () → ())%obsSig))
+            (SiR_hyp : exists SiR,
+                         (forall mutIdx,
+                            refineMutator SiR (getMutDef mutDefs mutIdx) (getMutDef mutDefs mutIdx))
+                         /\ (forall obsIdx,
+                               refineObserver SiR (getObsDef obsDefs obsIdx) (getObsDef obsDefs obsIdx))
+                         /\ refineObserver SiR
+                                           (obsBody (ith obsSig_eq obsDefs idx _
+                                                         (@Build_obsDef Rep ("null" : rep × () → ()) (fun r _ => ret tt))
+                                           ))
+                                           (obsBody newDef))
+  : refineADT
+      (BuildADT mutDefs obsDefs)
+      (ADTReplaceObsDef mutDefs obsDefs idx newDef).
+  Proof.
+    destruct SiR_hyp as [SiR [? [? ?] ] ].
+    intros; eapply refineADT_BuildADT_Rep with (SiR := SiR);
+    trivial.
+    intro obsIdx.
+    case_eq (obsSig_eq (nth (findIndex obsSig_eq obsSigs idx) obsSigs
+                            ("null" : rep × () → ())%obsSig) obsIdx);
+      intro H'.
+    - generalize (In_obsSigs_eq _ _ _ H'); intros; subst.
+      simpl; intros; erewrite ith_replace'; eauto.
+    - simpl replaceObsDef; simpl getObsDef; erewrite ith_replace; eauto.
+  Qed.
+
+  Lemma refineADT_BuildADT_ReplaceObserver_generic
+            (Rep : Type)
+            (mutSigs : list mutSig)
+            (obsSigs : list obsSig)
+            (mutDefs : ilist (@mutDef Rep) mutSigs)
+            (obsDefs : ilist (@obsDef Rep) obsSigs)
+            (idx : BoundedString (List.map obsID obsSigs))
+            (newDef : obsDef (nth (findIndex obsSig_eq obsSigs idx)
+                                  obsSigs ("null" : rep × () → ())%obsSig))
+            SiR
+            (SiR_reflexive_mutator : forall mutIdx,
+                                       refineMutator SiR (getMutDef mutDefs mutIdx) (getMutDef mutDefs mutIdx))
+            (SiR_reflexive_observer : forall obsIdx,
+                                        refineObserver SiR (getObsDef obsDefs obsIdx) (getObsDef obsDefs obsIdx))
+  : refineObserver SiR
+                   (obsBody (ith obsSig_eq obsDefs idx _
+                                 (@Build_obsDef Rep ("null" : rep × () → ()) (fun r _ => ret tt))
+                   ))
+                   (obsBody newDef)
     -> refineADT
          (BuildADT mutDefs obsDefs)
          (ADTReplaceObsDef mutDefs obsDefs idx newDef).
   Proof.
-    intros; eapply refineADT_BuildADT_Rep with (SiR := SiR); eauto.
-    intros; unfold getObsDef.
-    caseEq (obsSig_eq (nth (findIndex obsSig_eq obsSigs idx) obsSigs
-                           ("null" : rep × () → ())%obsSig) obsIdx).
-    - generalize (In_obsSigs_eq _ _ _ H2); intros; subst.
-      simpl; intros; erewrite ith_replace'; eauto.
-    - simpl replaceObsDef; erewrite ith_replace; eauto.
+    intros.
+    eapply refineADT_BuildADT_ReplaceObserver_generic_ex; repeat (eassumption || esplit).
+  Qed.
+
+  Lemma refineADT_BuildADT_ReplaceObserver
+            (Rep : Type)
+            (mutSigs : list mutSig)
+            (obsSigs : list obsSig)
+            (mutDefs : ilist (@mutDef Rep) mutSigs)
+            (obsDefs : ilist (@obsDef Rep) obsSigs)
+            (idx : BoundedString (List.map obsID obsSigs))
+            (newDef : obsDef (nth (findIndex obsSig_eq obsSigs idx)
+                                  obsSigs ("null" : rep × () → ())%obsSig))
+  : refineObserver eq
+                   (obsBody (ith obsSig_eq obsDefs idx _
+                                 (@Build_obsDef Rep ("null" : rep × () → ()) (fun r _ => ret tt))
+                   ))
+                   (obsBody newDef)
+    -> refineADT
+         (BuildADT mutDefs obsDefs)
+         (ADTReplaceObsDef mutDefs obsDefs idx newDef).
+  Proof.
+    eapply refineADT_BuildADT_ReplaceObserver_generic;
+    reflexivity.
   Qed.
 
   Lemma refineADT_BuildADT_ReplaceObserver_eq
             (Rep : Type)
-            (SiR : Rep -> Rep -> Prop)
             (mutSigs : list mutSig)
             (obsSigs : list obsSig)
             (mutDefs : ilist (@mutDef Rep) mutSigs)
@@ -180,6 +232,30 @@ Section BuildADTRefinements.
   Proof.
     eapply refineADT_BuildADT_ReplaceObserver;
     simpl; unfold refine; intros; subst; eauto.
+  Qed.
+
+  Lemma refineADT_BuildADT_ReplaceObserver_sigma
+        (RepT : Type)
+        (RepInv : RepT -> Prop)
+        (mutSigs : list mutSig)
+        (obsSigs : list obsSig)
+        (mutDefs : ilist (@mutDef (sig RepInv)) mutSigs)
+        (obsDefs : ilist (@obsDef (sig RepInv)) obsSigs)
+        (idx : BoundedString (List.map obsID obsSigs))
+        (newDef : obsDef (nth (findIndex obsSig_eq obsSigs idx)
+                              obsSigs ("null" : rep × () → ())%obsSig))
+  : refineObserver (fun x y => proj1_sig x = proj1_sig y)
+                   (obsBody (ith obsSig_eq obsDefs idx _
+                                 (@Build_obsDef (sig RepInv) ("null" : rep × () → ()) (fun r _ => ret tt))
+                   ))
+                   (obsBody newDef)
+    -> refineADT
+         (BuildADT mutDefs obsDefs)
+         (ADTReplaceObsDef mutDefs obsDefs idx newDef).
+  Proof.
+    intro H'.
+    eapply refineADT_BuildADT_ReplaceObserver_eq.
+    simpl in *; intros; subst; eauto.
   Qed.
 
 End BuildADTRefinements.
